Remove obsolete benchmarks, add Wolfram sqrt benchmark.

src/misc/benchmarks_nobuild.v
@@ -1,99 +1,40 @@
 Require Import 
-  BigZ BigQ fast_integers nonneg_integers_naturals
-  fast_rationals
-  abstract_algebra interfaces.integers interfaces.rationals 
-  interfaces.additional_operations (* interfaces.appfield *)
-  dyadics (* dyadics_appfield *).
+  abstract_algebra interfaces.integers interfaces.additional_operations fast_integers.
 
-Check (_ : Integers fastZ).
-Check (_ : ∀ (x y : fastZ), Decision (x = y)).
-Check (_ : ∀ (x y : Pos fastZ), Decision (x = y)).
-Check (_ : ∀ (x y : fastZ), Decision (x ≤ y)).
-Check (_ : ∀ (x y : Pos fastZ), Decision (x ≤ y)).
-Check (_ : NatPow fastZ (Pos fastZ)).
-Check (_ : ShiftLeft fastZ (Pos fastZ)). 
-Check (_ : ShiftRight fastZ (Pos fastZ)). 
-Check (_ : RingMinus fastZ).
-Check (_ : CutMinus fastZ).
-Check (_ : Log (2:fastZ) (Pos fastZ)).
-Check (_ : DivEuclid fastZ).
-Check (_ : RingMinus fastZ).
-Check (_ : CutMinus fastZ).
-Check (_ : CutMinus (Pos fastZ)).
+Section wolfram_sqrt.
+Context `{Integers Z} `{!RingOrder oZ} `{!TotalOrder oZ}
+  `{precedes_dec : ∀ (x y : Z), Decision (x ≤ y)} `{!ShiftLSpec Z (Z⁺) sl}.
 
-Definition D : Dyadic fastZ := (233123124123412343%bigZ) $ (12314%bigZ).
-Definition E : Dyadic fastZ := (2151453412523525234%bigZ) $ (-13152%bigZ).
-Program Definition Y : fastZ⁺ := 256%bigZ.
-Next Obligation. Admitted.
-
-Time Eval vm_compute in (D + E).
-Time Eval vm_compute in ((D ✚ E) Y).
-
-Definition Q1 : fastQ := (1#3)%bigQ.
-
-Time Eval vm_compute in (QtoD Q1 Y).
-Time Eval vm_compute in (((QtoD Q1 Y) * (3%bigZ $ 0))).
-Time Eval vm_compute in (DtoQ (
-  ((QtoD Q1 Y) ✖ (3%bigZ $ 0)) Y
-)).
-Time Eval vm_compute in (Q1 * (3#1)%bigQ).
-Time Eval vm_compute in (((QtoD Q1 Y) ✖ (3%bigZ $ 0)) Y).
-Time Eval vm_compute in (DtoQ (
-  ((QtoD Q1 Y) ✚ (3%bigZ $ 0)) Y
-)).
-
-Definition DyadicNeZero := sig (λ z : Dyadic fastZ , z ≠ 0).
-
-Program Definition D2 : DyadicNeZero := D.
-Next Obligation.  Admitted.
-
-Program Definition Y2 : Pos fastZ := 45%bigZ.
-Next Obligation. Admitted.
-Eval vm_compute in ((/// D2) Y2).
-
-(* Ad hoc implementation of Euler *)
-Program Fixpoint euler_aux (x : Dyadic fastZ) (n : nat) (m : DyadicNeZero) (ε : Pos fastZ) {struct n} : Dyadic fastZ := 
-  match n with 
-  | O => 1
-  | S n' => 1 + (((x ✖ ((/// m) ε)) ε) ✖ (euler_aux x n' (exist _ (1 + proj1_sig m) _) ε)) ε
+Fixpoint root_loop (x : Z) (n : nat) : Z * Z :=
+  match n with
+  | O => (x, 0)
+  | S n => let (r, s) := root_loop x n in
+     if decide_rel (≤) (s + 1) r
+     then ((r - (s + 1)) ≪ 2, (s + 2) ≪ 1)
+     else (r ≪ 2, s ≪ 1)
   end.
-Next Obligation. Admitted.
+End wolfram_sqrt.
 
-Program Definition D3 : DyadicNeZero := (1:Dyadic fastZ).
-Next Obligation.  Admitted.
+Definition fast_root_loop := root_loop (Z:=fastZ).
 
-Program Definition Y3 : Pos fastZ := 90%bigZ.
-Next Obligation.  Admitted.
+Let n : nat := Eval vm_compute in (10 * 10 * 10 * 10)%nat.
 
-(* Extremely hacky way to display a dyadic in a readable way *)
-Program Definition answer (n : fastZ) (x : Dyadic fastZ) : fastZ :=
- div_euclid (mant x * (10%bigZ) ^ (int_abs fastZ (Pos fastZ) n)) (exist _ (1 ≪ int_abs fastZ (Pos fastZ) (expo x)) _).
-Next Obligation. Admitted.
+Time Eval vm_compute in (snd (fast_root_loop 2 n)).
+(* 7.432465s *)
 
-Time Eval vm_compute in (answer (20%bigZ) (euler_aux (euler_aux 2 50 D3 Y3) 50 D3 Y3)).
-Time Eval vm_compute in (answer (20%bigZ) (euler_aux (euler_aux (euler_aux (1$(-1%bigZ)) 45 D3 Y3) 45 D3 Y3) 45 D3 Y3)).
+Require Import BigZ.
+Open Scope bigZ_scope.
 
-Definition fastQNeZero := sig (λ z : fastQ, z ≠ 0).
-
-Program Fixpoint eulerQ_aux (x : fastQ) (n : nat) (m : fastQNeZero) {struct n} : fastQ := 
-  match n return fastQ with 
-  | O => 1
-  | S n' => 1 + x * ((eulerQ_aux x n' (exist _ (1 + proj1_sig m) _)) // m)
+Fixpoint root_loop_alt (x : bigZ) (n : nat) : bigZ * bigZ :=
+  match n with
+  | O => (x, 0)
+  | S n => let (r, s) := root_loop_alt x n in
+     match BigZ.compare (s + 1) r with
+     | Gt => (BigZ.shiftl r 2, BigZ.shiftl s 1)
+     | _ => (BigZ.shiftl (r - (s + 1)) 2, BigZ.shiftl (s + 2) 1)
+     end
   end.
-Next Obligation. Admitted.
 
-Time Eval vm_compute in (eulerQ_aux (eulerQ_aux 2 300 1) 300 1).
+Time Eval vm_compute in (snd (root_loop_alt 2 n)).
+(* 7.264454s *)
 
-Check (_ : Integers Z).
-Check (_ : ∀ (x y : Z), Decision (x = y)).
-Check (_ : ∀ (x y : Z), Decision (x ≤ y)).
-Check (_ : NatPow Z (Pos Z)).
-Check (_ : ShiftLeft Z (Pos Z)). 
-Check (_ : RingMinus Z).
-Check (_ : CutMinus Z).
-
-Definition DZ : Dyadic Z := (233123124123412343%Z) $ (12314%Z).
-Definition EZ : Dyadic Z := (2151453412523525234%Z) $ (-13152%Z).
-Time Eval vm_compute in (DZ + EZ).
-
-(* log2 and div_euclid aren't implemented for Z yet, so we can't test ✚ *)
